src/Distributions/Uniform/Model.dfy
@@ -51,14 +51,15 @@ module Uniform.Model {
     }
     var e := iset s | Loops.ProposalIsAccepted(Proposal(n), Accept(n))(s);
     assert e in Rand.eventSpace by {
-      assert e == Measures.PreImage(s => UniformPowerOfTwo.Model.Sample(2 * n)(s).value, (iset m: nat | m < n));
-      assert Measures.PreImage(s => UniformPowerOfTwo.Model.Sample(2 * n)(s).value, (iset m: nat | m < n)) in Rand.eventSpace by {
+      assert e == Measures.PreImage(UniformPowerOfTwo.Model.Sample(2 * n), (iset r: Monad.Result<nat> | r.Result? && r.value < n));
+      assert Measures.PreImage(UniformPowerOfTwo.Model.Sample(2 * n), (iset r: Monad.Result<nat> | r.Result? && r.value < n)) in Rand.eventSpace by {
         assert Independence.IsIndep(UniformPowerOfTwo.Model.Sample(2 * n)) by {
           UniformPowerOfTwo.Correctness.SampleIsIndep(2 * n);
         }
-        assert Measures.IsMeasurable(Rand.eventSpace, Measures.natEventSpace, s => UniformPowerOfTwo.Model.Sample(2 * n)(s).value) by {
-          Independence.IsIndepImpliesValueMeasurableNat(UniformPowerOfTwo.Model.Sample(2 * n));
+        assert Measures.IsMeasurable(Rand.eventSpace, Monad.ResultEventSpace(Measures.natEventSpace), UniformPowerOfTwo.Model.Sample(2 * n)) by {
+          Independence.IsIndepImpliesMeasurableNat(UniformPowerOfTwo.Model.Sample(2 * n));
         }
+        assert (iset r: Monad.Result<nat> | r.Result? && r.value < n) in Monad.ResultEventSpace(Measures.natEventSpace);
       }
     }
     assert Quantifier.WithPosProb(Loops.ProposalIsAccepted(Proposal(n), Accept(n))) by {
